src/Invariant.v
@@ -69,6 +69,74 @@ Section Invariant.
   
 End Invariant.
 
+Section MutualInvariant.
+  Variables (SystemI StateI LabelI: Type).
+  Context `{HasInit SystemI StateI} `{HasLabel LabelI}.
+
+  Variable (impl: SystemI).
+
+  Variables (stepI: Step SystemI StateI LabelI)
+            (inv1 inv2: StateI -> Prop).
+
+  Definition MutualInvStep1 :=
+    forall ist1,
+      Reachable (steps stepI) impl ist1 ->
+      inv1 ist1 -> inv2 ist1 ->
+      forall lbl ist2,
+        stepI impl ist1 lbl ist2 ->
+        inv1 ist2.
+
+  Definition MutualInvStep2 :=
+    forall ist1,
+      Reachable (steps stepI) impl ist1 ->
+      inv1 ist1 -> inv2 ist1 ->
+      forall lbl ist2,
+        stepI impl ist1 lbl ist2 ->
+        inv2 ist2.
+
+  Hypotheses (Hminvi1: InvInit impl inv1)
+             (Hminvi2: InvInit impl inv2)
+             (Hminvs1: MutualInvStep1)
+             (Hminvs2: MutualInvStep2).
+
+  Lemma mutual_inv_steps':
+    forall ist1,
+      Reachable (steps stepI) impl ist1 ->
+      inv1 ist1 -> inv2 ist1 ->
+      forall ihst ist2,
+        steps stepI impl ist1 ihst ist2 ->
+        inv1 ist2 /\ inv2 ist2.
+  Proof.
+    induction 4; simpl; intros; eauto.
+    split.
+    - eapply Hminvs1 with (ist1:= st2); eauto.
+      + eapply reachable_steps; eauto.
+      + apply IHsteps; auto.
+      + apply IHsteps; auto.
+    - eapply Hminvs2 with (ist1:= st2); eauto.
+      + eapply reachable_steps; eauto.
+      + apply IHsteps; auto.
+      + apply IHsteps; auto.
+  Qed.
+
+  Lemma mutual_inv_steps:
+    InvSteps impl stepI (fun st => inv1 st /\ inv2 st).
+  Proof.
+    unfold InvSteps; intros.
+    eapply mutual_inv_steps'; eauto.
+    apply reachable_init.
+  Qed.
+
+  Corollary mutual_inv_reachable:
+    InvReachable impl stepI (fun st => inv1 st /\ inv2 st).
+  Proof.
+    unfold InvReachable; intros.
+    destruct H1 as [ll ?].
+    eapply mutual_inv_steps; eauto.
+  Qed.
+
+End MutualInvariant.
+
 Section Operations.
   Context {StateT: Type}.
 
