src/Ex/Mesi/MesiSim.v
@@ -460,8 +460,6 @@ Section Sim.
           apply getDir_ME_imp in H; destruct H
         end.
 
-  Hypothesis (Hmftinv: InvReachable impl step_m (MesiFootprintsInv topo)).
-
   Theorem mesi_sim_ok:
     InvSim step_m step_m (MesiInv.InvForSim topo) SimMESI impl spec.
   Proof.
@@ -1110,7 +1108,7 @@ Section Sim.
       { (* [liDownSRsUpDownME] *)
         disc_rule_conds_ex; spec_case_silent.
         derive_footprint_info_basis oidx;
-          [|disc_mesi_footprints_inv oidx H27].
+          [|disc_MesiDownLockInv oidx H27].
         derive_child_chns upCIdx.
         derive_child_idx_in upCIdx.
         disc_responses_from.
@@ -1126,7 +1124,7 @@ Section Sim.
       { (* liDownSRsUpDownS] *)
         disc_rule_conds_ex; spec_case_silent.
         derive_footprint_info_basis oidx;
-          [|disc_mesi_footprints_inv oidx H27].
+          [|disc_MesiDownLockInv oidx H27].
         derive_child_chns upCIdx.
         derive_child_idx_in upCIdx.
         disc_responses_from.
@@ -1163,7 +1161,7 @@ Section Sim.
       { (* [liDownSRsUpUp] *)
         disc_rule_conds_ex; spec_case_silent.
         derive_footprint_info_basis oidx;
-          [disc_mesi_footprints_inv oidx H27|].
+          [disc_MesiDownLockInv oidx H27|].
         disc_responses_from.
         derive_child_chns cidx.
         derive_child_idx_in cidx.
@@ -1192,7 +1190,7 @@ Section Sim.
       { (* [liDownIRsUpDown] *)
         disc_rule_conds_ex; spec_case_silent.
         derive_footprint_info_basis oidx;
-          [|disc_mesi_footprints_inv oidx H27].
+          [|disc_MesiDownLockInv oidx H27].
         derive_child_chns upCIdx.
         derive_child_idx_in upCIdx.
         disc_responses_from.
@@ -1223,7 +1221,7 @@ Section Sim.
       { (* [liDownIRsUpUp] *)
         disc_rule_conds_ex; spec_case_silent.
         derive_footprint_info_basis oidx;
-          [disc_mesi_footprints_inv oidx H27|].
+          [disc_MesiDownLockInv oidx H27|].
         disc_responses_from.
         solve_sim_mesi.
       }
